fix min_positive and change spec to linked list

src/examples/implang_cont_eg.v
@@ -4,16 +4,16 @@ From iris_simp_lang Require Import implang_cont imp_cont_notation lifting_expr l
 Local Open Scope func_scope.
 
 (* Returns the minimum positive integer, or #0 if there isn't one.
-  l: address of head of an array *)
+  l: pointer to a linked list or null, each cell is (value, ptr_to_next_cell) *)
 Definition min_positive :=
   fn "l" <{ ( "min" "v" )
     "min" <a- #0 ;;
     While !"l" ≠ #0 <{
-      If !"l" < !"min" <{ break }> <{ skip }>;;
+      (* If !"l" < !"min" <{ break }> ;; *)
       "v" <a- !"l";;
       "l" <a- !("l" + #1);;
-      If "v" <= #0 <{ continue }> <{ skip }>;;
-      If "min" = #0 || "v" < "min" <{ "min" <a- "v" }> <{ skip }>
+      If "v" <= #0 <{ continue }> ;;
+      If "min" = #0 || "v" < "min" <{ "min" <a- "v" }> 
     }>;;
     Return "min"
   }>.
@@ -25,6 +25,8 @@ Section spec.
 
   Context `{!gen_heapGS loc val Σ} `{!envGS val Σ} `{!invGS_gen HasNoLc Σ}.
 
+  Local Open Scope bi_scope.
+
   Definition min_positive_r (lv: list Z) : Z :=
     foldr Z.min 0%Z lv.
 
@@ -32,18 +34,28 @@ Section spec.
     (l + i)%Z.
   Notation "l +ₗ i" := (ptr_add l i) (at level 10, left associativity).
 
-  (* a list of [0;1;...; (n-1)] *)
-  Definition indices n := map (Z.of_nat) (seq 0%nat n).
-  Definition array_points_to (l: loc) (lv: list Z) : assert :=
-    ([∗ list] i; v ∈ indices (length lv); lv, (l +ₗ i) ↦ (NumV v))%I.
-  Instance array_points_to_objective l lv : Objective (array_points_to l lv).
+  (* a linked list starting with l and stores lv; tail pointer is `last` *)
+  Fixpoint llist_seg (l: loc) (lv: list Z) (last: loc) : assert :=
+    match lv with
+    | [] => ⌜l = last⌝
+    | v :: lv' => ∃ l', l ↦ NumV v ∗ (l+ₗ1) ↦ LocV l' ∗ llist_seg l' lv' last
+    end.
+
+  Definition llist (l: loc) (lv: list Z) := llist_seg l lv 0%Z.
+
+  Global Instance llist_seg_objective l lv last : Objective (llist_seg l lv last).
   Proof.
-    rewrite /array_points_to. generalize (indices (length lv)).
-    induction lv => indices.
-    - destruct indices; simpl; apply _.
-    - destruct indices; simpl; apply _.
+    generalize l.
+    induction lv => ?; apply _.
   Qed.
-  Notation "l ↦ₐ lv" := (array_points_to l lv) (at level 10) : bi_scope.
+  Global Instance llist_objective l lv : Objective (llist l lv).
+  Proof.
+    generalize l.
+    induction lv => ?; apply _.
+  Qed.
+
+  Notation "l ↦ₛ lv" := (llist_seg l lv) (at level 9) : bi_scope.
+  Notation "l ↦ₗ lv" := (llist l lv) (at level 10) : bi_scope.
 
 
   (* FIXME make this into a lemma up1_fupd *)
@@ -58,14 +70,21 @@ Section spec.
   Ltac iSteps := repeat first [iStep | iModIntro | progress iFrame | progress iIntros ].
 
   Lemma min_positive_spec E (l: loc) (lv: list Z) z :
-    (∃ _z, "r" ↦v NumV _z) ∗ l ↦ₐ lv
-    ⊢ call_assert F E min_positive [LocV l; NumV 0; NumV 0] "r" ("r" ↦v NumV z ∗ l ↦ₐ lv ∗ ⌜min_positive_r lv = z⌝).
+    (∃ _z, "r" ↦v NumV _z) ∗ l ↦ₗ lv
+    ⊢ call_assert F E min_positive [LocV l; NumV 0; NumV 0] "r" ("r" ↦v NumV z ∗ l ↦ₗ lv ∗ ⌜min_positive_r lv = z⌝).
   Proof.
     iIntros "((%_z & r) & arr)".
     wp_start_func with_retainer "retainer" and_locals "(l & min & v & _)".
     iSteps.
     simpl.
-    wp_apply wp_while; simpl.
+
+    set (∃ l_m lv_a lv_b, ⌜lv = lv_a++lv_b⌝ ∧ l ↦ₛ lv_a l_m ∗ l_m ↦ₗ lv_b ∗
+                "l" ↦v (LocV l_m) ∗ "v" ↦v (NumV (min_positive_r lv_a)))%I%Z as inv.
+    wp_apply (wp_while_inv  _ _ _ _ inv with "[] [-r retainer]" ) ; simpl.
+    {
+      iIntros "!> (%l_m & %lv_a & %lv_b & %Hlv & arr_a & arr_b & l & v)".
+      { iSteps. 
+      
   Admitted.
 
 End spec.
